books/centaur/gl/bfr.lisp
@@ -34,88 +34,73 @@
 (include-book "centaur/ubdds/lite" :dir :system)
 (include-book "centaur/ubdds/param" :dir :system)
 (include-book "centaur/aig/misc" :dir :system)
-(include-book "std/basic/defs" :dir :system)
 (local (include-book "centaur/aig/aig-vars" :dir :system))
 (local (include-book "centaur/misc/arith-equivs" :dir :system))
 
-(defstub bfr-mode () t)
-(defun bfr-aig () (declare (xargs :guard t)) t)
-(defun bfr-bdd () (declare (xargs :guard t)) nil)
+(defsection bfr
+  :parents (reference)
+  :short "An abstraction of the <b>B</b>oolean <b>F</b>unction
+<b>R</b>epresentation used by GL."
 
-;; Default to using BDDs
-(defattach bfr-mode bfr-bdd)
+  :long "<p>GL was originally designed to operate on @(see ubdds), with
+support for @(see aig)s being added later.  To avoid redoing a lot of proof
+work, a small level of indirection was added.</p>
 
-(defmacro bfr-case (&key aig bdd)
-  `(if (bfr-mode)
-       ,aig ,bdd))
+<p>The particular Boolean function representation that we are using at any
+particular time is governed by @(see bfr-mode), and operations like @(see
+bfr-and) allow us to construct new function nodes using whatever the current
+representation is.</p>")
 
-;; (defmacro bfr-event (&key aig bdd)
-;;   `(make-event
-;;     (if *experimental-aig-mode*
-;;         ',aig ',bdd)))
+(local (xdoc::set-default-parents bfr))
 
+;; [Jared]: Note that I deleted a lot of old commented-out code relating to
+;; defining bfr-p and proving related things about bfr-p.  I think that idea
+;; has been long abandoned.  If you ever want to review it, you can go back to
+;; Git revision 1207333ab8e09e338b7216c473c8f6654410c360 or earlier.
+
+(defsection bfr-mode
+  :short "Determine the current @(see bfr) mode we are using."
+  :long "<p>GL users should generally not use this.</p>
+
+<p>@(call bfr-mode) is an attachable function which is typically attached to
+either @('bfr-aig') or @('bfr-bdd').  When it returns true, we are to use @(see
+aig)s, otherwise we use @(see ubdds).</p>
+
+@(def bfr-mode)"
+
+  (defstub bfr-mode () t)
+  (defun bfr-aig () (declare (xargs :guard t)) t)
+  (defun bfr-bdd () (declare (xargs :guard t)) nil)
+
+  ;; Default to using BDDs
+  (defattach bfr-mode bfr-bdd))
+
+(defsection bfr-case
+  :short "Choose behavior based on the current @(see bfr) mode."
+  :long "<p>Usage:</p>
+
+@({
+     (brf-case :aig aigcode
+               :bdd bddcode)
+})
+
+<p>expands to @('aigcode') if we are currently in AIG mode, or @('bddcode') if
+we are currently in BDD mode.  This is often used to implement basic wrappers
+like @(see bfr-and).</p>
+
+@(def bfr-case)"
+
+  (defmacro bfr-case (&key aig bdd)
+    `(if (bfr-mode)
+         ,aig
+       ,bdd)))
 
 (local (in-theory (enable booleanp)))
 
-;; (defun bfr-p (x)
-;;   (declare (xargs :guard t)
-;;            (ignorable x))
-;;   (mbe :logic
-;;        (bfr-case :bdd (acl2::ubddp x) :aig t)
-;;        :exec (or (booleanp x)
-;;                  (bfr-case :bdd (acl2::ubddp x) :aig t))))
 
-;; (defthm bfr-p-booleanp
-;;   (booleanp (bfr-p x))
-;;   :rule-classes :type-prescription)
-
-
-;; (defthmd bfr-p-of-boolean
-;;   (implies (booleanp x) (bfr-p x))
-;;   :hints (("goal" :in-theory (enable bfr-p acl2::ubddp))))
-
-;; (defun bfr-fix (x)
-;;   (declare (xargs :guard t))
-;;   (mbe :logic
-;;        (bfr-case :bdd (acl2::ubdd-fix x) :aig x)
-;;        :exec
-;;        (if (booleanp x)
-;;            x
-;;          (bfr-case :bdd (acl2::ubdd-fix x) :aig x))))
-
-;; (defthm bfr-p-bfr-fix
-;;   (bfr-p (bfr-fix x)))
-
-;; (defthm bfr-fix-when-bfr-p
-;;   (implies (bfr-p x)
-;;            (equal (bfr-fix x) x)))
-
-
-;; (defun bfr-equiv (a b)
-;;   (equal (bfr-fix a) (bfr-fix b)))
-
-;; (defequiv bfr-equiv)
-
-;; (defthm bfr-fix-bfr-equiv
-;;   (bfr-equiv (bfr-fix x) x))
-
-;; (defmacro bfrfix (x)
-;;   `(mbe :logic (bfr-fix ,x) :exec ,x))
-
-;; (defun bfr-fix-bindings (vars)
-;;   (if (atom vars)
-;;       nil
-;;     (cons `(,(car vars) (bfrfix ,(car vars)))
-;;           (bfr-fix-bindings (cdr vars)))))
-
-;; (defmacro bfr-fix-vars (vars body)
-;;   `(let ,(bfr-fix-bindings vars)
-;;      (declare (ignorable . ,vars))
-;;      ,body))
-
-
-(defun bfr-eval (x env)
-  (declare (xargs :guard t))
+(define bfr-eval (x env)
+  :short "Evaluate a BFR under an appropriate BDD/AIG environment."
+  :returns bool
   (mbe :logic
        (bfr-case :bdd (acl2::eval-bdd x env)
                  :aig (acl2::aig-eval x env))
@@ -123,22 +108,84 @@
        (if (booleanp x)
            x
          (bfr-case :bdd (acl2::eval-bdd x env)
-                   :aig (acl2::aig-eval x env)))))
+                   :aig (acl2::aig-eval x env))))
+  ///
+  (defthm bfr-eval-consts
+    (and (equal (bfr-eval t env) t)
+         (equal (bfr-eval nil env) nil))))
 
-;; (defthmd bfr-eval-of-bfr-fix
-;;   (equal (bfr-eval (bfr-fix x) env)
-;;          (bfr-eval x env))
-;;   :hints (("goal" :use acl2::eval-bdd-ubdd-fix
-;;            :in-theory (disable acl2::eval-bdd-ubdd-fix))))
 
-;; (defcong bfr-equiv equal (bfr-eval x env) 1
-;;   :hints (("goal" :use ((:instance bfr-eval-of-bfr-fix)
-;;                         (:instance bfr-eval-of-bfr-fix
-;;                                    (x x-equiv)))
-;;            :in-theory (disable bfr-eval bfr-fix))))
+(defsection bfr-equiv
+  :short "Semantics equivalence of BFRs, i.e., equal evaluation under every
+possible environment."
 
-(defun bfr-not (x)
-  (declare (xargs :guard t))
+  (acl2::def-universal-equiv bfr-equiv
+    :qvars (env)
+    :equiv-terms ((equal (bfr-eval acl2::x env))))
+
+  (defcong bfr-equiv equal (bfr-eval x env) 1
+    :hints(("Goal" :in-theory (e/d (bfr-equiv-necc))))))
+
+
+(define bfr-lookup ((n natp) env)
+  :short "Look up a BFR variable in an appropriate BDD/AIG environment."
+  (let ((n (lnfix n)))
+    (bfr-case
+      :bdd (and (acl2::with-guard-checking nil (ec-call (nth n env))) t)
+      :aig (let ((look (hons-get n env)))
+             (if look
+                 (and (cdr look) t)
+               t))))
+  ///
+  (in-theory (disable (:e bfr-lookup)))
+
+  (defcong acl2::nat-equiv equal (bfr-lookup n env) 1
+    :hints(("Goal" :in-theory (enable bfr-lookup)))))
+
+
+(define bfr-set-var ((n natp) val env)
+  :short "Set the @('n')th BFR variable to some value in an AIG/BDD environment."
+  (let ((n (lnfix n)))
+    (bfr-case :bdd (acl2::with-guard-checking
+                    nil
+                    (ec-call (update-nth n (and val t) env)))
+              :aig (hons-acons n (and val t) env)))
+  ///
+  (in-theory (disable (:e bfr-set-var)))
+
+  (defthm bfr-lookup-bfr-set-var
+    (equal (bfr-lookup n (bfr-set-var m val env))
+           (if (equal (nfix n) (nfix m))
+               (and val t)
+             (bfr-lookup n env)))
+    :hints(("Goal" :in-theory (e/d (bfr-lookup bfr-set-var)
+                                   (update-nth nth)))))
+
+  (defcong acl2::nat-equiv equal (bfr-set-var n val env) 1
+    :hints(("Goal" :in-theory (enable bfr-set-var)))))
+
+
+(define bfr-var ((n natp))
+  :short "Construct the @('n')th BFR variable."
+  (let ((n (lnfix n)))
+    (bfr-case :bdd (acl2::qv n)
+              :aig n))
+  ///
+  (in-theory (disable (:e bfr-var)))
+
+  (defthm bfr-eval-bfr-var
+    (equal (bfr-eval (bfr-var n) env)
+           (bfr-lookup n env))
+    :hints(("Goal" :in-theory (enable bfr-lookup bfr-eval bfr-var
+                                      acl2::eval-bdd))))
+
+  (defcong acl2::nat-equiv equal (bfr-var n) 1
+    :hints(("Goal" :in-theory (enable bfr-var)))))
+
+
+(define bfr-not (x)
+  :short "Construct the NOT of a BFR."
+  :returns (bfr)
   (mbe :logic
        (bfr-case :bdd (acl2::q-not x)
                  :aig (acl2::aig-not x))
@@ -146,25 +193,23 @@
        (if (booleanp x)
            (not x)
          (bfr-case :bdd (acl2::q-not x)
-                   :aig (acl2::aig-not x)))))
+                   :aig (acl2::aig-not x))))
+  ///
+  (defthm bfr-eval-bfr-not
+    (equal (bfr-eval (bfr-not x) env)
+           (not (bfr-eval x env)))
+    :hints(("Goal" :in-theory (enable bfr-eval))))
 
-;; (defthm bfr-p-bfr-not
-;;   (bfr-p (bfr-not x)))
+  (local (in-theory (disable bfr-not)))
 
-;; (local (acl2::add-bdd-fn-pat acl2::ubdd-fix))
-
-(defthm bfr-eval-bfr-not
-  (equal (bfr-eval (bfr-not x) env)
-         (not (bfr-eval x env)))
-  :hints (("goal" :in-theory (enable booleanp))))
-
-;;(defcong bfr-equiv bfr-equiv (bfr-not x) 1)
-
-(in-theory (disable bfr-not))
+  (defcong bfr-equiv bfr-equiv (bfr-not x) 1
+    :hints ((and stable-under-simplificationp
+                 `(:expand (,(car (last clause))))))))
 
 
-(defun bfr-binary-and (x y)
-  (declare (xargs :guard t))
+(define bfr-binary-and (x y)
+  :parents (bfr-and)
+  :returns (bfr)
   (mbe :logic
        (bfr-case :bdd (acl2::q-binary-and x y)
                  :aig (acl2::aig-and x y))
@@ -173,34 +218,33 @@
              ((not y) nil)
              ((and (eq x t) (eq y t)) t)
              (t (bfr-case :bdd (acl2::q-binary-and x y)
-                          :aig (acl2::aig-and x y))))))
+                          :aig (acl2::aig-and x y)))))
+  ///
+  (defthm bfr-eval-bfr-binary-and
+    (equal (bfr-eval (bfr-binary-and x y) env)
+           (and (bfr-eval x env)
+                (bfr-eval y env)))
+    :hints (("goal" :in-theory (e/d (bfr-eval) ((force))))))
 
-;; (defthm bfr-p-bfr-binary-and
-;;   (bfr-p (bfr-binary-and x y)))
+  (defthm bfr-and-of-nil
+    (and (equal (bfr-binary-and nil y) nil)
+         (equal (bfr-binary-and x nil) nil))
+    :hints(("Goal" :in-theory (enable acl2::aig-and))))
 
-(defthm bfr-eval-bfr-binary-and
-  (equal (bfr-eval (bfr-binary-and x y) env)
-         (and (bfr-eval x env)
-              (bfr-eval y env)))
-  :hints (("goal" :in-theory (e/d (booleanp) ((force))))))
+  (local (in-theory (disable bfr-binary-and)))
 
-(defthm bfr-and-of-nil
-  (and (equal (bfr-binary-and nil y) nil)
-       (equal (bfr-binary-and x nil) nil))
-  :hints(("Goal" :in-theory (enable acl2::aig-and))))
+  (defcong bfr-equiv bfr-equiv (bfr-binary-and x y) 1
+    :hints ((and stable-under-simplificationp
+                 `(:expand (,(car (last clause)))))))
 
+  (defcong bfr-equiv bfr-equiv (bfr-binary-and x y) 2
+    :hints ((and stable-under-simplificationp
+                 `(:expand (,(car (last clause))))))))
 
-
-;; (defcong bfr-equiv equal (bfr-binary-and a b) 1)
-
-;; (defcong bfr-equiv equal (bfr-binary-and a b) 2)
-
-(in-theory (disable bfr-binary-and))
-
-
-(defun bfr-and-macro-logic-part (args)
-  ;; Generates the :logic part for a bfr-and MBE call.
-  (declare (xargs :mode :program))
+(define bfr-and-macro-logic-part (args)
+  :parents (bfr-and)
+  :short "Generates the :logic part for a bfr-and MBE call."
+  :mode :program
   (cond ((atom args)
          t)
         ((atom (cdr args))
@@ -208,9 +252,10 @@
         (t
          `(bfr-binary-and ,(car args) ,(bfr-and-macro-logic-part (cdr args))))))
 
-(defun bfr-and-macro-exec-part (args)
-  ;; Generates the :exec part for a bfr-and MBE call.
-  (declare (xargs :mode :program))
+(define bfr-and-macro-exec-part (args)
+  :parents (bfr-and)
+  :short "Generates the :exec part for a bfr-and MBE call."
+  :mode :program
   (cond ((atom args)
          t)
         ((atom (cdr args))
@@ -224,16 +269,17 @@
                    (bfr-and-x-do-not-use-elsewhere)
                    ,(bfr-and-macro-exec-part (cdr args)))))))))
 
-(defmacro bfr-and (&rest args)
-  `(mbe :logic ,(bfr-and-macro-logic-part args)
-        :exec  ,(bfr-and-macro-exec-part  args)))
+(defsection bfr-and
+  :short "@('(bfr-and x1 x2 ...)') constructs the AND of these BFRs."
+  :long "@(def bfr-and)"
+  (defmacro bfr-and (&rest args)
+    `(mbe :logic ,(bfr-and-macro-logic-part args)
+          :exec  ,(bfr-and-macro-exec-part  args))))
 
 
-
-
-
-(defun bfr-ite-fn (x y z)
-  (declare (xargs :guard t))
+(define bfr-ite-fn (x y z)
+  :parents (bfr-ite)
+  :returns (bfr)
   (mbe :logic
        (bfr-case :bdd (acl2::q-ite x y z)
                  :aig (cond ((eq x t) y)
@@ -245,47 +291,54 @@
          (bfr-case :bdd (acl2::q-ite x y z)
                    :aig (cond ((eq x t) y)
                               ((eq x nil) z)
-                              (t (acl2::aig-ite x y z)))))))
+                              (t (acl2::aig-ite x y z))))))
+  ///
+  (defthm bfr-eval-bfr-ite-fn
+    (equal (bfr-eval (bfr-ite-fn x y z) env)
+           (if (bfr-eval x env)
+               (bfr-eval y env)
+             (bfr-eval z env)))
+    :hints (("goal" :in-theory (enable booleanp bfr-eval))))
 
-;; (defthm bfr-p-bfr-ite-fn
-;;   (bfr-p (bfr-ite-fn x y z)))
+  (defthm bfr-ite-fn-bools
+    (and (equal (bfr-ite-fn t y z) y)
+         (equal (bfr-ite-fn nil y z) z)))
 
-(defthm bfr-eval-bfr-ite-fn
-  (equal (bfr-eval (bfr-ite-fn x y z) env)
-         (if (bfr-eval x env)
-             (bfr-eval y env)
-           (bfr-eval z env)))
-  :hints (("goal" :in-theory (enable booleanp))))
+  (local (in-theory (disable bfr-ite-fn)))
 
-(defthm bfr-ite-fn-bools
-  (and (equal (bfr-ite-fn t y z) y)
-       (equal (bfr-ite-fn nil y z) z)))
+  (defcong bfr-equiv bfr-equiv (bfr-ite-fn x y z) 1
+    :hints ((and stable-under-simplificationp
+                 `(:expand (,(car (last clause)))))))
 
+  (defcong bfr-equiv bfr-equiv (bfr-ite-fn x y z) 2
+    :hints ((and stable-under-simplificationp
+                 `(:expand (,(car (last clause)))))))
 
-;; (defcong bfr-equiv equal (bfr-ite-fn x y z) 1)
-;; (defcong bfr-equiv equal (bfr-ite-fn x y z) 2)
-;; (defcong bfr-equiv equal (bfr-ite-fn x y z) 3)
-
-(in-theory (disable bfr-ite-fn))
-
-
-(defmacro bfr-ite (x y z)
-  (cond ((and (or (quotep y) (atom y))
-              (or (quotep z) (atom z)))
-         `(bfr-ite-fn ,x ,y ,z))
-        (t
-         `(mbe :logic (bfr-ite-fn ,x ,y ,z)
-               :exec (let ((bfr-ite-x-do-not-use-elsewhere ,x))
-                       (cond
-                        ((eq bfr-ite-x-do-not-use-elsewhere nil) ,z)
-                        ((eq bfr-ite-x-do-not-use-elsewhere t) ,y)
-                        (t
-                         (bfr-ite-fn bfr-ite-x-do-not-use-elsewhere
-                                     ,y ,z))))))))
+  (defcong bfr-equiv bfr-equiv (bfr-ite-fn x y z) 3
+    :hints ((and stable-under-simplificationp
+                 `(:expand (,(car (last clause))))))))
 
 
-(defun bfr-binary-or (x y)
-  (declare (xargs :guard t))
+(defsection bfr-ite
+  :short "@(call bfr-ite) constructs the If-Then-Else of these BFRs."
+  :long "@(def bfr-ite)"
+  (defmacro bfr-ite (x y z)
+    ;; BOZO why not move the COND inside the ITE?
+    (cond ((and (or (quotep y) (atom y))
+                (or (quotep z) (atom z)))
+           `(bfr-ite-fn ,x ,y ,z))
+          (t
+           `(mbe :logic (bfr-ite-fn ,x ,y ,z)
+                 :exec (let ((bfr-ite-x-do-not-use-elsewhere ,x))
+                         (cond
+                          ((eq bfr-ite-x-do-not-use-elsewhere nil) ,z)
+                          ((eq bfr-ite-x-do-not-use-elsewhere t) ,y)
+                          (t
+                           (bfr-ite-fn bfr-ite-x-do-not-use-elsewhere
+                                       ,y ,z)))))))))
+
+(define bfr-binary-or (x y)
+  :parents (bfr-or)
   (mbe :logic
        (bfr-case :bdd (acl2::q-or x y)
                  :aig (acl2::aig-or x y))
@@ -293,33 +346,34 @@
        (if (and (booleanp x) (booleanp y))
            (or x y)
          (bfr-case :bdd (acl2::q-or x y)
-                   :aig (acl2::aig-or x y)))))
+                   :aig (acl2::aig-or x y))))
+  ///
+  (defthm bfr-eval-bfr-binary-or
+    (equal (bfr-eval (bfr-binary-or x y) env)
+           (or (bfr-eval x env)
+               (bfr-eval y env)))
+    :hints (("goal" :in-theory (e/d (booleanp bfr-eval) ((force))))))
 
-;; (defthm bfr-p-bfr-binary-or
-;;   (bfr-p (bfr-binary-or x y)))
+  (defthm bfr-or-of-t
+    (and (equal (bfr-binary-or t y) t)
+         (equal (bfr-binary-or y t) t))
+    :hints(("Goal" :in-theory (enable acl2::aig-or
+                                      acl2::aig-and
+                                      acl2::aig-not))))
 
-(defthm bfr-eval-bfr-binary-or
-  (equal (bfr-eval (bfr-binary-or x y) env)
-         (or (bfr-eval x env)
-             (bfr-eval y env)))
-  :hints (("goal" :in-theory (e/d (booleanp) ((force))))))
+  (local (in-theory (disable bfr-binary-or)))
 
-(defthm bfr-or-of-t
-  (and (equal (bfr-binary-or t y) t)
-       (equal (bfr-binary-or y t) t))
-  :hints(("Goal" :in-theory (enable acl2::aig-or
-                                    acl2::aig-and
-                                    acl2::aig-not))))
+  (defcong bfr-equiv bfr-equiv (bfr-binary-or x y) 1
+    :hints ((and stable-under-simplificationp
+                 `(:expand (,(car (last clause)))))))
 
-;; (defcong bfr-equiv equal (bfr-binary-or x y) 1)
-;; (defcong bfr-equiv equal (bfr-binary-or x y) 2)
+  (defcong bfr-equiv bfr-equiv (bfr-binary-or x y) 2
+    :hints ((and stable-under-simplificationp
+                 `(:expand (,(car (last clause))))))))
 
-(in-theory (disable bfr-binary-or))
-
-
-
-(defun bfr-or-macro-logic-part (args)
-  (declare (xargs :mode :program))
+(define bfr-or-macro-logic-part (args)
+  :parents (bfr-or)
+  :mode :program
   (cond ((atom args)
          nil)
         ((atom (cdr args))
@@ -327,8 +381,9 @@
         (t
          `(bfr-binary-or ,(car args) ,(bfr-or-macro-logic-part (cdr args))))))
 
-(defun bfr-or-macro-exec-part (args)
-  (declare (xargs :mode :program))
+(define bfr-or-macro-exec-part (args)
+  :parents (bfr-or)
+  :mode :program
   (cond ((atom args)
          nil)
         ((atom (cdr args))
@@ -347,15 +402,17 @@
                 (bfr-or-x-do-not-use-elsewhere)
                 ,(bfr-or-macro-exec-part (cdr args)))))))))
 
-(defmacro bfr-or (&rest args)
-  `(mbe :logic ,(bfr-or-macro-logic-part args)
-        :exec  ,(bfr-or-macro-exec-part  args)))
+(defsection bfr-or
+  :short "@('(bfr-or x1 x2 ...)') constructs the OR of these BFRs."
+  :long "@(def bfr-or)"
+
+  (defmacro bfr-or (&rest args)
+    `(mbe :logic ,(bfr-or-macro-logic-part args)
+          :exec  ,(bfr-or-macro-exec-part  args))))
 
 
-
-
-(defun bfr-xor (x y)
-  (declare (xargs :guard t))
+(define bfr-xor (x y)
+  :short "@(call bfr-xor) constructs the XOR of these BFRs."
   (mbe :logic
        (bfr-case :bdd (acl2::q-xor x y)
                  :aig (acl2::aig-xor x y))
@@ -363,28 +420,27 @@
        (if (and (booleanp x) (booleanp y))
            (xor x y)
          (bfr-case :bdd (acl2::q-xor x y)
-                   :aig (acl2::aig-xor x y)))))
+                   :aig (acl2::aig-xor x y))))
+  ///
+  (defthm bfr-eval-bfr-xor
+    (equal (bfr-eval (bfr-xor x y) env)
+           (xor (bfr-eval x env)
+                (bfr-eval y env)))
+    :hints (("goal" :in-theory (e/d (bfr-eval) ((force))))))
 
-;; (defthm bfr-p-bfr-xor
-;;   (bfr-p (bfr-xor x y)))
+  (local (in-theory (disable bfr-xor)))
 
-(defthm bfr-eval-bfr-xor
-  (equal (bfr-eval (bfr-xor x y) env)
-         (xor (bfr-eval x env)
-              (bfr-eval y env)))
-  :hints (("goal" :in-theory (e/d (booleanp) ((force))))))
+  (defcong bfr-equiv bfr-equiv (bfr-xor x y) 1
+    :hints ((and stable-under-simplificationp
+                 `(:expand (,(car (last clause)))))))
 
-;; (defcong bfr-equiv equal (bfr-xor x y) 1
-;;   :hints(("Goal" :in-theory (enable booleanp))))
-;; (defcong bfr-equiv equal (bfr-xor x y) 2
-;;   :hints(("Goal" :in-theory (enable booleanp))))
-
-(in-theory (disable bfr-xor))
+  (defcong bfr-equiv bfr-equiv (bfr-xor x y) 2
+    :hints ((and stable-under-simplificationp
+                 `(:expand (,(car (last clause))))))))
 
 
-
-(defun bfr-iff (x y)
-  (declare (xargs :guard t))
+(define bfr-iff (x y)
+  :short "@(call bfr-iff) constructs the IFF of these BFRs."
   (mbe :logic
        (bfr-case :bdd (acl2::q-iff x y)
                  :aig (acl2::aig-iff x y))
@@ -392,94 +448,24 @@
        (if (and (booleanp x) (booleanp y))
            (iff x y)
          (bfr-case :bdd (acl2::q-iff x y)
-                   :aig (acl2::aig-iff x y)))))
+                   :aig (acl2::aig-iff x y))))
+  ///
+  (defthm bfr-eval-bfr-iff
+    (equal (bfr-eval (bfr-iff x y) env)
+           (iff (bfr-eval x env)
+                (bfr-eval y env)))
+    :hints (("goal" :in-theory (e/d (bfr-eval) ((force))))))
 
-;; (defthm bfr-p-bfr-iff
-;;   (bfr-p (bfr-iff x y)))
+  (local (in-theory (disable bfr-iff)))
 
-(defthm bfr-eval-bfr-iff
-  (equal (bfr-eval (bfr-iff x y) env)
-         (iff (bfr-eval x env)
-              (bfr-eval y env)))
-  :hints (("goal" :in-theory (e/d (booleanp) ((force))))))
+  (defcong bfr-equiv bfr-equiv (bfr-iff x y) 1
+    :hints ((and stable-under-simplificationp
+                 `(:expand (,(car (last clause)))))))
 
+  (defcong bfr-equiv bfr-equiv (bfr-iff x y) 2
+    :hints ((and stable-under-simplificationp
+                 `(:expand (,(car (last clause))))))))
 
-;; (defcong bfr-equiv equal (bfr-iff x y) 1
-;;   :hints(("Goal" :in-theory (enable booleanp))))
-;; (defcong bfr-equiv equal (bfr-iff x y) 2
-;;   :hints(("Goal" :in-theory (enable booleanp))))
-
-(in-theory (disable bfr-iff))
-
-
-(defthm bfr-eval-consts
-  (and (equal (bfr-eval t env) t)
-       (equal (bfr-eval nil env) nil)))
-
-
-
-;; (in-theory (disable bfr-eval bfr-fix bfr-p
-;;                     (:type-prescription bfr-p)))
-
-
-(defun bfr-var (n)
-  (declare (xargs :guard (natp n)))
-  (let ((n (lnfix n)))
-    (bfr-case :bdd (acl2::qv n)
-              :aig n)))
-
-;; (defthm bfr-p-bfr-var
-;;   (bfr-p (bfr-var n))
-;;   :hints(("Goal" :in-theory (enable bfr-p))))
-
-(in-theory (disable bfr-var (bfr-var)))
-
-
-(defun  bfr-lookup (n env)
-  (declare (xargs :guard (natp n)))
-  (let ((n (lnfix n)))
-    (bfr-case :bdd (and (acl2::with-guard-checking nil (ec-call (nth n env))) t)
-              :aig (let ((look (hons-get n env)))
-                     (if look
-                         (and (cdr look) t)
-                       t)))))
-
-(defthm bfr-eval-bfr-var
-  (equal (bfr-eval (bfr-var n) env)
-         (bfr-lookup n env))
-  :hints(("Goal" :in-theory (enable bfr-lookup bfr-eval bfr-var
-                                    acl2::eval-bdd))))
-
-(in-theory (disable bfr-lookup (bfr-lookup)))
-
-
-(defun bfr-set-var (n val env)
-  (declare (xargs :guard (natp n)))
-  (let ((n (lnfix n)))
-    (bfr-case :bdd (acl2::with-guard-checking
-                    nil
-                    (ec-call (update-nth n (and val t) env)))
-              :aig (hons-acons n (and val t) env))))
-
-(defthm bfr-lookup-bfr-set-var
-  (equal (bfr-lookup n (bfr-set-var m val env))
-         (if (equal (nfix n) (nfix m))
-             (and val t)
-           (bfr-lookup n env)))
-  :hints(("Goal" :in-theory (e/d (bfr-lookup bfr-set-var)
-                                 (update-nth nth)))))
-
-(in-theory (disable bfr-set-var (bfr-set-var) bfr-eval))
-
-
-(defcong acl2::nat-equiv equal (bfr-var n) 1
-  :hints(("Goal" :in-theory (enable bfr-var))))
-
-(defcong acl2::nat-equiv equal (bfr-lookup n env) 1
-  :hints(("Goal" :in-theory (enable bfr-lookup))))
-
-(defcong acl2::nat-equiv equal (bfr-set-var n val env) 1
-  :hints(("Goal" :in-theory (enable bfr-set-var))))
 
 
 
@@ -487,11 +473,6 @@
 ;;++++++++++++++++++++++++++++++++++++++++++++++++++++++++++++++++++++
 ;; BFR reasoning clause processor
 ;;++++++++++++++++++++++++++++++++++++++++++++++++++++++++++++++++++++
-
-(include-book "clause-processors/term-patterns" :dir :system)
-(include-book "clause-processors/join-thms" :dir :system)
-
-
 
 (defmacro bfr-patterns ()
   '(acl2::get-term-patterns bfr))
@@ -513,17 +494,18 @@
 
 (set-bfr-patterns nil)
 
-(add-bfr-fn-pats
- bfr-binary-and bfr-not bfr-binary-or bfr-xor bfr-iff bfr-ite-fn
- bfr-fix)
+(add-bfr-fn-pats bfr-binary-and
+                 bfr-not
+                 bfr-binary-or
+                 bfr-xor
+                 bfr-iff
+                 bfr-ite-fn)
 
 (add-bfr-pats 't 'nil)
 
 (defun bfr-termp (x bfr-terms pats)
   (or (member-equal x bfr-terms)
       (acl2::match-term-pattern x pats)))
-
-
 
 (defmacro bfr-eval-patterns ()
   '(acl2::get-term-patterns bfr-eval))
@@ -541,15 +523,14 @@
 
 (add-bfr-eval-pats (bfr-eval & env))
 
-
 (defevaluator bfr-cp-ev bfr-cp-evl
-  ((bfr-eval a b) (equal a b) (not a)
+  ((bfr-eval a b)
+   (equal a b)
+   (not a)
    (implies a b)
    (if a b c)))
 
 (acl2::def-join-thms bfr-cp-ev)
-
-
 
 (mutual-recursion
  (defun collect-bfr-eval-vals (term patterns)
@@ -565,8 +546,6 @@
      (union-equal (collect-bfr-eval-vals (car clause) patterns)
                   (collect-bfr-eval-vals-list (cdr clause) patterns)))))
 
-
-(include-book "tools/flag" :dir :system)
 (flag::make-flag collect-bfr-eval-vals-flag collect-bfr-eval-vals
                  :flag-mapping ((collect-bfr-eval-vals . term)
                                 (collect-bfr-eval-vals-list . list)))
@@ -581,7 +560,6 @@
   (list (implies (pseudo-term-listp clause)
                  (pseudo-term-listp (collect-bfr-eval-vals-list clause patterns))))
   :hints (("goal" :induct (collect-bfr-eval-vals-flag flag term clause patterns))))
-
 
 (defun bfr-eval-vals (clause patterns)
   (let ((collect (collect-bfr-eval-vals-list clause patterns)))
@@ -715,7 +693,6 @@
                         cphint)))))
      (value nil)))
 
-
 (defmacro bfr-reasoning-mode (flg)
   (if flg
       '(add-default-hints '((bfr-reasoning)))
@@ -723,61 +700,7 @@
 
 
 
-(acl2::def-universal-equiv
- bfr-equiv
- :qvars (env)
- :equiv-terms ((equal (bfr-eval acl2::x env))))
 
-(defcong bfr-equiv equal (bfr-eval x env) 1
-  :hints(("Goal" :in-theory (e/d (bfr-equiv-necc)))))
-
-(defcong bfr-equiv bfr-equiv (bfr-not x) 1
-  :hints ((and stable-under-simplificationp
-               `(:expand (,(car (last clause)))))))
-
-(defcong bfr-equiv bfr-equiv (bfr-and x y) 1
-  :hints ((and stable-under-simplificationp
-               `(:expand (,(car (last clause)))))))
-
-(defcong bfr-equiv bfr-equiv (bfr-and x y) 2
-  :hints ((and stable-under-simplificationp
-               `(:expand (,(car (last clause)))))))
-
-(defcong bfr-equiv bfr-equiv (bfr-or x y) 1
-  :hints ((and stable-under-simplificationp
-               `(:expand (,(car (last clause)))))))
-
-(defcong bfr-equiv bfr-equiv (bfr-or x y) 2
-  :hints ((and stable-under-simplificationp
-               `(:expand (,(car (last clause)))))))
-
-(defcong bfr-equiv bfr-equiv (bfr-xor x y) 1
-  :hints ((and stable-under-simplificationp
-               `(:expand (,(car (last clause)))))))
-
-(defcong bfr-equiv bfr-equiv (bfr-xor x y) 2
-  :hints ((and stable-under-simplificationp
-               `(:expand (,(car (last clause)))))))
-
-(defcong bfr-equiv bfr-equiv (bfr-iff x y) 1
-  :hints ((and stable-under-simplificationp
-               `(:expand (,(car (last clause)))))))
-
-(defcong bfr-equiv bfr-equiv (bfr-iff x y) 2
-  :hints ((and stable-under-simplificationp
-               `(:expand (,(car (last clause)))))))
-
-(defcong bfr-equiv bfr-equiv (bfr-ite x y z) 1
-  :hints ((and stable-under-simplificationp
-               `(:expand (,(car (last clause)))))))
-
-(defcong bfr-equiv bfr-equiv (bfr-ite x y z) 2
-  :hints ((and stable-under-simplificationp
-               `(:expand (,(car (last clause)))))))
-
-(defcong bfr-equiv bfr-equiv (bfr-ite x y z) 3
-  :hints ((and stable-under-simplificationp
-               `(:expand (,(car (last clause)))))))
 
 
 
